\documentclass{article}
\usepackage{amsmath}
\usepackage[a4paper, total={6in,10in}]{geometry}

\begin{document}
\huge

$$
P = \begin{bmatrix} 0 \\ 1\end{bmatrix} \text{- sākumpunkts}
$$

$$
T = \begin{bmatrix} T_x \\ T_y\end{bmatrix} \text {- mērķis}
$$

$$ 
R(\Theta) = \begin{bmatrix} cos \Theta & -sin \Theta \\ sin \Theta & cos \Theta \end{bmatrix}
$$

$$
R'(\Theta) = \begin{bmatrix}-sin \Theta & -cos \Theta\\cos \Theta & -sin \Theta\end{bmatrix}
$$

$$
d(\Theta _ 1, \Theta _ 2) = R(\Theta_1)P+R(\Theta_1)(R(\Theta_2)P)-T
$$

$$
\frac{ \partial d(\Theta_1, \Theta_2)}{\partial \Theta_1} = R'(\Theta_1)P +  R'(\Theta_1)(R(\Theta_2)P)
$$

$$
f(\Theta _ 1, \Theta _ 2) = \frac{d(\Theta _ 1, \Theta _ 2)^2}{2}
$$
\begin{multline*}
\frac{\partial f(\Theta _ 1, \Theta _ 2)}{\partial \Theta_1} = \frac {\partial (\frac{1}{2}d(\Theta _ 1, \Theta _ 2)^2)}{\partial \Theta_1} =\\ \\
\frac {\partial (\frac{1}{2}d(\Theta _ 1, \Theta _ 2)^2)}{\partial d(\Theta _ 1, \Theta _ 2)} \cdot \frac{ \partial d(\Theta_1, \Theta_2)}{\partial \Theta_1}
= \\ \\ d(\Theta _ 1, \Theta _ 2) \cdot (R'(\Theta_1)P +  R'(\Theta_1)(R(\Theta_2)P))
\end{multline*
}
\end{document}
